# Bicubic Image Interpolation


### System of Equations
```
a00 = f(1,1)
a01 = -0.5*f(1,0) + 0.5*f(1,2)
a02 = f(1,0) - 2.5*f(1,1) + 2*f(1,2) - 0.5*f(1,3)
a03 = -0.5*f(1,0) + 1.5*f(1,1) - 1.5*f(1,2) + 0.5*f(1,3)
a10 = -0.5*f(0,1) + 0.5*f(2,1)
a11 = 0.25*f(0,0) - 0.25*f(0,2) - 0.25*f(2,0) + 0.25*f(2,2)
a12 = -.5*f(0,0) + 1.25*f(0,1) - f(0,2) + .25*f(0,3) + .5*f(2,0) - 1.25*f(2,1) + f(2,2) -.25*f(2,3)
a13 = .25*f(0,0) - .75*f(0,1) + .75*f(0,2) - .25*f(0,3) - .25*f(2,0) + .75*f(2,1) - .75*f(2,2) + .25*f(2,3)
a20 = f(0,1) - 2.5*f(1,1) + 2*f(2,1) - .5*f(3,1)
a21 = -.5*f(0,0) + .5*f(0,2) + 1.25*f(1,0) - 1.25*f(1,2) - f(2,0) + f(2,2) + .25*f(3,0) - .25*f(3,2)
a22 = f(0,0) - 2.5*f(0,1) + 2*f(0,2) - .5*f(0,3) - 2.5*f(1,0) + 6.25*f(1,1) - 5*f(1,2) + 1.25*f(1,3) + 2*f(2,0) - 5*f(2,1) + 4*f(2,2) - f(2,3) - .5*f(3,0) + 1.25*f(3,1) - f(3,2) + .25*f(3,3)
a23 = -.5*f(0,0) + 1.5*f(0,1) - 1.5*f(0,2) + .5*f(0,3) + 1.25*f(1,0) - 3.75*f(1,1) + 3.75*f(1,2) - 1.25*f(1,3) - f(2,0) + 3*f(2,1) - 3*f(2,2) + f(2,3) + .25*f(3,0) - .75*f(3,1) + .75*f(3,2) - .25*f(3,3)
a30 = -.5*f(0,1) + 1.5*f(1,1) - 1.5*f(2,1) + .5*f(3,1)
a31 = .25*f(0,0) - .25*f(0,2) - .75*f(1,0) + .75*f(1,2) + .75*f(2,0) - .75*f(2,2) - .25*f(3,0) + .25*f(3,2)
a32 = -.5*f(0,0) + 1.25*f(0,1) - f(0,2) + .25*f(0,3) + 1.5*f(1,0) - 3.75*f(1,1) + 3*f(1,2) - .75*f(1,3) - 1.5*f(2,0) + 3.75*f(2,1) - 3*f(2,2) + .75*f(2,3) + .5*f(3,0) - 1.25*f(3,1) + f(3,2) - .25*f(3,3)
a33 = .25*f(0,0) - .75*f(0,1) + .75*f(0,2) - .25*f(0,3) - .75*f(1,0) + 2.25*f(1,1) - 2.25*f(1,2) + .75*f(1,3) + .75*f(2,0) - 2.25*f(2,1) + 2.25*f(2,2) - .75*f(2,3) - .25*f(3,0) + .75*f(3,1) - .75*f(3,2) + .25*f(3,3) 
```

### General Form
```
f(x,y) = (a00 + a01 * y + a02 * y2 + a03 * y3) +
(a10 + a11 * y + a12 * y2 + a13 * y3) * x +
(a20 + a21 * y + a22 * y2 + a23 * y3) * x2 +
(a30 + a31 * y + a32 * y2 + a33 * y3) * x3
```